prove conversion between big_sepM over addr and (addr2flat addr)
required strengthening flatid_addr_map

src/program_proof/addr/specs.v
@@ -90,9 +90,8 @@ Section flatid2addr.
   Variable (T : Type).
 
   Definition flatid_addr_map (fm : gmap u64 T) (am : gmap addr T) : Prop :=
-    ∀ (a : addr) (v : T),
-      valid_addr a ->
-      am !! a = Some v <-> fm !! (addr2flat a) = Some v.
+    ( ∀ a v, am !! a = Some v -> valid_addr a ∧ fm !! (addr2flat a) = Some v ) ∧
+    ( ∀ fa v, fm !! fa = Some v -> ∃ a, valid_addr a ∧ addr2flat a = fa ∧ am !! a = Some v ).
 
   Theorem flatid_addr_lookup fm am a :
     flatid_addr_map fm am ->
@@ -103,7 +102,10 @@ Section flatid2addr.
     destruct (am !! a) eqn:Heq.
     - apply H; eauto.
     - destruct (fm !! addr2flat a) eqn:Heq2; eauto.
-      apply H in Heq2; eauto. congruence.
+      apply H in Heq2; eauto.
+      destruct Heq2; intuition idtac.
+      apply addr2flat_eq in H1; eauto; subst.
+      congruence.
   Qed.
 
   Theorem flatid_addr_insert fm am a v :
@@ -111,11 +113,85 @@ Section flatid2addr.
     valid_addr a ->
     flatid_addr_map (<[addr2flat a := v]> fm) (<[a := v]> am).
   Proof.
-    rewrite /flatid_addr_map /valid_addr; intros.
-    destruct (decide (a = a0)); subst.
-    - repeat rewrite lookup_insert; eauto.
-    - rewrite -> lookup_insert_ne by eauto.
-      rewrite -> lookup_insert_ne by (apply addr2flat_ne; eauto).
+    rewrite /flatid_addr_map; split; intros.
+    - destruct (decide (a = a0)); subst.
+      + rewrite lookup_insert in H1; inversion H1; clear H1; subst.
+        repeat rewrite -> lookup_insert; eauto.
+      + rewrite -> lookup_insert_ne in H1 by eauto.
+        apply H in H1; intuition eauto.
+        rewrite -> lookup_insert_ne by (apply addr2flat_ne; eauto).
+        eauto.
+    - destruct (decide (addr2flat a = fa)); subst.
+      + rewrite lookup_insert in H1; inversion H1; clear H1; subst.
+        eexists.
+        repeat rewrite -> lookup_insert; eauto.
+      + rewrite -> lookup_insert_ne in H1 by eauto.
+        apply H in H1; destruct H1. intuition eauto.
+        exists x; intuition eauto.
+        rewrite -> lookup_insert_ne; eauto.
+        congruence.
+  Qed.
+
+  Theorem flatid_addr_insert_inv_2 fm am a v :
+    flatid_addr_map fm (<[a := v]> am) ->
+      valid_addr a ∧
+      fm !! (addr2flat a) = Some v ∧
+      flatid_addr_map (delete (addr2flat a) fm) (delete a am).
+  Proof.
+    intros.
+    destruct H.
+    edestruct H.
+    { erewrite lookup_insert; eauto. }
+    intuition eauto.
+    split; intros.
+    - destruct (decide (a = a0)); subst.
+      { rewrite lookup_delete in H3; congruence. }
+      rewrite lookup_delete_ne in H3; eauto.
+      edestruct H.
+      { rewrite lookup_insert_ne; eauto. }
+      intuition eauto.
+      rewrite lookup_delete_ne; eauto.
+      eapply addr2flat_ne; eauto.
+    - destruct (decide (addr2flat a = fa)); subst.
+      { rewrite lookup_delete in H3; congruence. }
+      rewrite lookup_delete_ne in H3; eauto.
+      apply H0 in H3. destruct H3.
+      exists x. intuition eauto.
+      rewrite -> lookup_insert_ne in H6 by congruence.
+      rewrite -> lookup_delete_ne by congruence.
+      eauto.
+  Qed.
+
+  Theorem flatid_addr_insert_inv_1 fm am fa v :
+    flatid_addr_map (<[fa := v]> fm) am ->
+    ∃ a,
+      valid_addr a ∧
+      fa = addr2flat a ∧
+      am !! a = Some v ∧
+      flatid_addr_map (delete fa fm) (delete a am).
+  Proof.
+    intros.
+    destruct H.
+    edestruct H0.
+    { erewrite lookup_insert; eauto. }
+    exists x.
+    intuition eauto.
+    split; intros.
+    - destruct (decide (a = x)); subst.
+      { rewrite lookup_delete in H3; congruence. }
+      rewrite lookup_delete_ne in H3; eauto.
+      edestruct H; eauto.
+      intuition eauto.
+      rewrite -> lookup_insert_ne in H5 by (apply addr2flat_ne; eauto).
+      rewrite lookup_delete_ne; eauto.
+      eapply addr2flat_ne; eauto.
+    - destruct (decide (fa = fa0)); subst.
+      { rewrite lookup_delete in H3; congruence. }
+      rewrite lookup_delete_ne in H3; eauto.
+      edestruct H0.
+      { rewrite lookup_insert_ne; eauto. }
+      exists x0; intuition eauto.
+      rewrite -> lookup_delete_ne by congruence.
       eauto.
   Qed.
 
@@ -124,23 +200,112 @@ Section flatid2addr.
     valid_addr a ->
     flatid_addr_map (delete (addr2flat a) fm) (delete a am).
   Proof.
-    rewrite /flatid_addr_map /valid_addr; intros.
-    destruct (decide (a = a0)); subst.
-    - repeat rewrite lookup_delete; eauto.
-    - rewrite -> lookup_delete_ne by eauto.
-      rewrite -> lookup_delete_ne by (apply addr2flat_ne; eauto).
-      eauto.
+    rewrite /flatid_addr_map; split; intros.
+    - destruct (decide (a = a0)); subst.
+      + rewrite lookup_delete in H1; congruence.
+      + rewrite -> lookup_delete_ne in H1 by eauto.
+        apply H in H1; intuition eauto.
+        rewrite -> lookup_delete_ne by (apply addr2flat_ne; eauto).
+        eauto.
+    - destruct (decide (addr2flat a = fa)); subst.
+      + rewrite lookup_delete in H1; congruence.
+      + rewrite -> lookup_delete_ne in H1 by eauto.
+        apply H in H1; destruct H1.
+        exists x; intuition eauto.
+        rewrite lookup_delete_ne; eauto.
+        congruence.
   Qed.
 
   Theorem flatid_addr_empty :
     flatid_addr_map ∅ ∅.
   Proof.
-    unfold flatid_addr_map; simpl; intros.
-    repeat rewrite lookup_empty.
-    eauto.
+    unfold flatid_addr_map; split; intros.
+    - rewrite lookup_empty in H; congruence.
+    - rewrite lookup_empty in H; congruence.
+  Qed.
+
+  Theorem flatid_addr_empty_1 m :
+    flatid_addr_map ∅ m -> m = ∅.
+  Proof.
+    unfold flatid_addr_map; intros.
+    apply map_empty; intros.
+    destruct (m !! i) eqn:He; eauto.
+    apply H in He. rewrite lookup_empty in He. intuition congruence.
+  Qed.
+
+  Theorem flatid_addr_empty_2 m :
+    flatid_addr_map m ∅ -> m = ∅.
+  Proof.
+    unfold flatid_addr_map; intros.
+    apply map_empty; intros.
+    destruct (m !! i) eqn:He; eauto.
+    apply H in He. destruct He. rewrite lookup_empty in H0. intuition congruence.
   Qed.
 
 End flatid2addr.
+
+
+Section map.
+  Context {PROP : bi}.
+  Context `{Countable K} {A : Type}.
+
+  Theorem big_sepM_flatid_addr_map_1 (Φ : _ -> A -> PROP) fm am :
+    flatid_addr_map fm am ->
+    ([∗ map] a↦b ∈ am, Φ a b) -∗ [∗ map] fa↦b ∈ fm, ∃ a, ⌜ fa = addr2flat a ⌝ ∗ Φ a b.
+  Proof.
+    rewrite <- (list_to_map_to_list am).
+    pose proof (NoDup_fst_map_to_list am); revert H0.
+    generalize (map_to_list am); intros l H0.
+    clear am; intros.
+    iIntros "H".
+
+    iInduction l as [|] "IH" forall (fm H0 H1).
+    - simpl in *. apply flatid_addr_empty_2 in H1. rewrite H1.
+      repeat rewrite big_sepM_empty. done.
+    - simpl in *. inversion H0; clear H0; subst.
+      apply flatid_addr_insert_inv_2 in H1; intuition idtac.
+      iDestruct (big_sepM_insert_delete with "H") as "[Ha H]".
+      erewrite <- (insert_id fm) by eauto.
+      iApply big_sepM_insert_delete.
+      iSplitL "Ha".
+      { iExists _; iFrame. done. }
+      rewrite delete_notin.
+      2: { apply not_elem_of_list_to_map_1; eauto. }
+      rewrite -> (delete_notin (list_to_map _)) in H3.
+      2: { apply not_elem_of_list_to_map_1; eauto. }
+      iDestruct ("IH" $! _ H5 H3 with "H") as "H".
+      iFrame.
+  Qed.
+
+  Theorem big_sepM_flatid_addr_map_2 (Φ : _ -> A -> PROP) fm am :
+    flatid_addr_map fm am ->
+    ([∗ map] fa↦b ∈ fm, Φ fa b) -∗ [∗ map] a↦b ∈ am, Φ (addr2flat a) b.
+  Proof.
+    rewrite <- (list_to_map_to_list fm).
+    pose proof (NoDup_fst_map_to_list fm); revert H0.
+    generalize (map_to_list fm); intros l H0.
+    clear fm; intros.
+    iIntros "H".
+
+    iInduction l as [|] "IH" forall (am H0 H1).
+    - simpl in *. apply flatid_addr_empty_1 in H1. rewrite H1.
+      repeat rewrite big_sepM_empty. done.
+    - simpl in *. inversion H0; clear H0; subst.
+      apply flatid_addr_insert_inv_1 in H1; destruct H1; intuition subst.
+      iDestruct (big_sepM_insert_delete with "H") as "[Ha H]".
+      erewrite <- (insert_id am) by eauto.
+      iApply big_sepM_insert_delete.
+      iSplitL "Ha".
+      { rewrite H0. iFrame. }
+      rewrite delete_notin.
+      2: { apply not_elem_of_list_to_map_1; eauto. }
+      rewrite -> (delete_notin (list_to_map _)) in H6.
+      2: { apply not_elem_of_list_to_map_1; eauto. }
+      iDestruct ("IH" $! _ H5 H6 with "H") as "H".
+      iFrame.
+  Qed.
+
+End map.
 
 
 Hint Unfold block_bytes : word.
